Progress on effect/handler rules

coq-osiris/theories/program_logic/rules.v
@@ -10,14 +10,110 @@ From osiris.lang Require Import lang.
 From osiris.program_logic Require Import ewp.
 From osiris.semantics Require Import step code.
 
+(* Local tactics for [ewp] rules *)
+(* LATER: move to a separate file *)
+Module ewp_rules_tactics.
+
+  Ltac ewp_unfold_all :=
+    rewrite !ewp_unfold /ewp_pre /=.
+  (* This tactic unfolds one occurrence of [ewp] at the head of the goal. *)
+  Ltac ewp_unfold_head :=
+    iApply ewp_unfold; rewrite /ewp_pre /=.
+
+  (* ------------------------------------------------------------------------ *)
+  (* Working with the state interpretation invariant. *)
+
+  (* [intro_state] introduces [σ] and [state_interp σ]. *)
+
+  Ltac intro_state := iIntros (σ) "Hsi".
+
+  (* -------------------------------------------------------------------------- *)
+  (** * Modality and mask (fupd) tactics *)
+
+  (* The Iris [wp] has mask-changing updates in order to enforce that during
+      a step of computation, no invariants can be opened. In order to control
+    the introduction of this mask change, and restore the mask, we provide
+    custom tactics analogous to "iModIntro" (here, [wp_mask_intro) and
+      "iMod [H]" (here, [wp_mask_elim]) (where [H] corresponds to a premise with
+      mask-changing information that restores the previous mask *)
+
+  (* Introduce a mask when there is a goal of shape (fupd E1 E2 _)
+      (i.e. The starting goal is of shape ⊢ |={E1, E2}=> P
+            and the updated goal is ⊢ P , where (|={E2, E1}=> emp) is introduced
+            as a premise)
+
+    The first mask [E1] indicates the set of invariants that can be opened
+    currently (i.e. before taking the mask-changing update) and the second mask
+    [E2] indicates the set of invariants that can be opened after the mask
+    change.
+
+    This tactic (through [fupd_mask_intro]) behaves as an "iModIntro" for
+    mask-changing updates and introduce a premise of shape (fupd E1 E2 emp).
+    This premise can be used later to restore the mask [E1] *)
+
+  Ltac ewp_mask_intro Hmod :=
+    iApply fupd_mask_intro; [ set_solver | ]; iIntros Hmod.
+
+  (* Try to introduce modalities "as much as possible" *)
+  Ltac try_iModIntro :=
+    repeat iModIntro; try iNext; repeat iModIntro.
+
+  (* Try to "cleanup" the goal; remove any modalities from the premise that can
+    be discharged trivially and then introduce any "straight forward" modalities
+    that can be introduced *)
+  Ltac ewp_cleanup_mod :=
+    repeat match goal with
+      | |- context[environments.Esnoc _
+                    ?Hmod (fupd empty empty _)] =>
+          iMod Hmod
+      end;
+    try_iModIntro.
+
+
+  Ltac ewp_mask_elim :=
+    ewp_cleanup_mod;
+    match goal with
+    | |- environments.envs_entails _ (fupd ?mask1 ?mask2 _) =>
+      try match goal with
+        | |- context[environments.Esnoc _ ?Hmod (fupd mask1 mask2 emp)] =>
+            iMod Hmod as "_"
+        end
+    end;
+    ewp_cleanup_mod.
+
+  (* ------------------------------------------------------------------------ *)
+  (* [intro_step] introduces [prim_step] along with the new expression and state *)
+  Ltac intro_step :=
+    let Hstep := fresh "Hstep" in
+    iIntros (???Hstep).
+
+  (* Discharge pure subgoal that follows immediately by [tac] *)
+  Tactic Notation "discharge_pure" tactic(tac) :=
+    match goal with
+    | |- environments.envs_entails _ (bi_sep (bi_pure _) _) =>
+        iSplitL ""; [ iPureIntro; by tac | ]
+    | |- environments.envs_entails _ (bi_sep  _ (bi_pure _)) =>
+        iSplitL ""; [ | iPureIntro; by tac ]
+    end.
+
+  Ltac construct_wp_nonret :=
+    (* Prove [can_step]: *)
+    (discharge_pure (auto with step can_step));
+    (* Introduce a hypothetical step: *)
+    intro_step.
+
+End ewp_rules_tactics.
+
 (* ------------------------------------------------------------------------ *)
 
 Section wp_rules.
 
-  Context `{!osirisGS Σ} `{protocol_wf Σ}.
+  Context `{!osirisGS Σ} `{protocol_wf Σ P}.
 
-  Context {X : Type}.
+  Context {A X : Type}.
+
   Implicit Type m : micro A X.
+  Import ewp_rules_tactics.
 
   (* Values *)
   Lemma ewp_value E Ψ Φ v :
@@ -34,6 +130,10 @@ Section wp_rules.
     EWP (Throw v : micro A X) @ E <| Ψ |> {{ Φ }} ={E}=∗ Φ (O2Throw v).
   Proof. Admitted.
 
+  Lemma ewp_crash_inv E Ψ Φ :
+    EWP (Crash : micro A X) @ E <| Ψ |> {{ Φ }} ={E}=∗ False.
+  Proof. Admitted.
+
   Lemma ewp_outcome2 E Ψ Φ v :
     Φ v -∗ EWP (inject2 v : micro A X) @ E <| Ψ |> {{ Φ }}.
   Proof. Admitted.
@@ -47,7 +147,7 @@ Section wp_rules.
 
   (* ------------------------------------------------------------------------ *)
   (** Monotonicity. *)
-  Lemma wp_covariant E m φ φ' Ψ:
+  Lemma ewp_mono E m φ φ' Ψ:
     EWP m @ E <| Ψ |> {{ φ }} -∗
     (∀ a, φ a -∗ φ' a) -∗
     EWP m @ E <| Ψ |> {{ φ' }}.
@@ -98,4 +198,122 @@ Section wp_rules.
   Proof. Admitted.
 
 End wp_rules.
+
+(* ------------------------------------------------------------------------ *)
+(* Invert cases where there are premises of the form
+          [EWP (ret _) _] [EWP crash _] or [EWP (throw _) _] *)
+Local Ltac ewp_invert :=
+  match goal with
+  | |- context [environments.Esnoc _ ?SI (state_interp _)] =>
+      match goal with
+      (* EWP throw *)
+      | |- context [environments.Esnoc _ ?Hwp (ewp_def _ (throw _) _ _)] =>
+          iPoseProof (ewp_throw_inv with "[$]") as "HΦ"
+      (* EWP ret *)
+      | |- context [environments.Esnoc _ ?Hwp (ewp_def _ (ret _) _ _)] =>
+          iMod (ewp_ret_inv with "[$]") as "HΦ"
+      (* EWP crash *)
+      | |- context [environments.Esnoc _ ?Hwp (ewp_def _ Crash _ _)] =>
+          iMod (ewp_crash_inv with "[$]") as "%"
+      end
+  end.
+(* ------------------------------------------------------------------------ *)
+
+(* Effect and handler rules *)
+
+Section wp_handler_rules.
+
+  Context `{!osirisGS Σ} `{protocol_wf Σ P}.
+
+  Context {A X : Type}.
+
+  Implicit Type m : micro A X.
+  Implicit Type Ψ : P.
+  Import ewp_rules_tactics.
+
+  Notation do v := (stop CPerform v).
+
+  Lemma ewp_do E Ψ v Φ:
+    prot_spec Ψ v Φ ⊢ EWP (do v) @ E <| Ψ |> {{ Φ }}.
+  Proof.
+    iIntros "HP".
+    ewp_unfold_head.
+    iApply prot_mono; iFrame.
+    iIntros (?) "HΦ". iNext.
+    by iApply ewp_outcome2.
+  Qed.
+
+  Lemma ewp_perform_inv {B X'} E Ψ v Φ (k : _ -> micro B X'):
+    EWP (Stop CPerform v k) @ E <| Ψ |> {{ Φ }} -∗
+    prot_spec Ψ v (fun w => ▷ EWP (k w) @ E <| Ψ |> {{ Φ }}).
+  Proof.
+    iIntros "HP".
+
+    ewp_unfold_all.
+    iApply prot_mono; iFrame.
+    iIntros (?) "HΦ". by iNext.
+  Qed.
+
+  Definition shallow_handler E Ψ Φ
+    (h : Outcome -> microvx) (* Handler for outcomes *)
+    (eh : Eff -> C.continuation -> microvx) (* Effect handler *)
+    Ψ' Φ' :=
+    ((∀ v, Φ v -∗ ▷ EWP (h v) @ E <| Ψ' |> {{ Φ' }}) ∧
+    (∀ v k l, prot_spec Ψ v (fun w => ▷ EWP (k w) @ E <| Ψ |> {{ Φ }}) -∗
+       mapsto l (DfracOwn 1) (K k) ==∗
+       ▷ EWP (eh v l) @ E <| Ψ' |> {{ Φ' }}))%I.
+
+  Definition handler (h : Outcome -> microvx) (eh : Eff -> C.continuation -> microvx) :
+    _ -> microvx :=
+    fun x =>
+      match x with
+        | O3Ret v => h (O2Ret v)
+        | O3Throw e => h (O2Throw e)
+        | O3Perform e c => eh e c
+      end.
+
+  (* Specification for handlers (shallow by default) *)
+  Lemma ewp_handler E Ψ Φ Ψ' Φ' e h eh:
+    EWP e @ E <| Ψ |> {{ Φ }} -∗
+    shallow_handler E Ψ Φ h eh Ψ' Φ' -∗
+    EWP (Handle e (handler h eh)) @ E <| Ψ' |> {{ Φ' }}.
+  Proof.
+    (* We proceed by Löb-induction after generalizing [e] [h] and [eh]. *)
+    iLöb as "IH" forall (e h eh).
+
+    iIntros "He Hsh".
+    ewp_unfold_head.
+    intro_state.
+
+    ewp_mask_intro "Hmod".
+    construct_wp_nonret; destruct_step; cbn; iMod "Hmod" as "_"; cbn.
+
+    1,2: (* [StepHandleRet] and [StepHandleThrow] *)
+      ewp_invert; iFrame;
+      iDestruct "Hsh" as "[Hsh _]";
+      iSpecialize ("Hsh" with "HΦ");
+      try iMod "Hsh";
+      by ewp_mask_intro "Hmod"; ewp_mask_elim.
+
+    { (* [StepHandlePerform] *)
+      iDestruct "Hsh" as "[_ Hsh]".
+      iPoseProof (ewp_perform_inv with "[$]") as "HP".
+      iSpecialize ("Hsh" $! _ _ with "HP").
+
+      iDestruct (gen_heap_alloc with "Hsi") as ">[Hsi [HH _]]"; first done.
+      iSpecialize ("Hsh" with "HH"). iMod "Hsh".
+
+      ewp_mask_intro "Hmod"; ewp_mask_elim.
+      iFrame. }
+
+    { (* [StepHandleCrash] *)
+      by ewp_invert. }
+
+    { (* [StepHandleLeft] *)
+
+      (* TODO: Need [ewp_step] *)
+
+  Admitted.
+
+End wp_handler_rules.
 
